semantics/primTypesScript.sml
@@ -33,7 +33,16 @@ Definition prim_sem_env_def:
   prim_sem_env (ffi:'ffi ffi_state) =
   add_to_sem_env
   (<|clock := 0; ffi := ffi; refs := []; next_type_stamp := 0;
-     next_exn_stamp := 0; eval_state := NONE|>,
+     next_exn_stamp := 0; eval_state := NONE;
+     fp_state := <|
+       rws := [];
+       opts := (λ x. []);
+       choices := 0;
+       canOpt := Strict;
+       assertions := (λ x y z. T);
+       real_sem := F;
+     |>
+   |>,
    <|v := nsEmpty; c := nsEmpty|>) prim_types_program
 End
 
